\subsection{Metodo di variazione delle costanti arbitrarie}
\[
    \underbrace{y' + a(x)y}_{(EO )} = f(x)
\]

\begin{enumerate}
    \item Si integra $(EO)$:
    \[ y(x) = C e^{-A(x)}  \mspace{15mu} C \in \R\]
    \item Serve una soluzione particolare:
    \[ y(x) = c(x) e^{-A(x)} \]
    \[ y'(x) = c'(x) e^{-A(x)} - c(x) e^{-A(x)} (a(x))\] 
    sostituendo in $y' + a(x)y = f(x)$:
    \[ c'(x) e^{-A(x)} - c(x) e^{-A(x)} (a(x)) + c(x) e^{-A(x)} = f(x)\]
    semplificando risulta:
    \[ c'(x) = e^{A(x)} f(x) \]
\end{enumerate}